theories/iris/logrel/path_defs.v
@@ -1,0 +1,32 @@
+Require Import stdpp.base.
+Require Import stdpp.list.
+Require Import stdpp.list_basics.
+Require Import RichWasm.syntax.
+Require Import RichWasm.typing.
+Require Import RichWasm.iris.memory.
+
+Definition get_path_words (off sz : nat) (ws : list word) : list word :=
+  firstn sz (skipn off ws).
+
+Definition update_path_words (off : nat) (ws ws' : list word) : list word :=
+  (firstn off ws) ++ ws' ++ (skipn (length ws') (skipn off ws)).
+
+Definition pr_expected (pr : path_result) (τ__π: option type) :=
+  match τ__π with
+  | Some τ__π' => τ__π'
+  | None => pr.(pr_target)
+  end.
+
+Lemma update_get_path_id off sz ws :
+  sz + off ≤ length ws ->
+  update_path_words off ws (get_path_words off sz ws) = ws.
+Proof.
+  etransitivity; last apply (take_drop off ws).
+  unfold update_path_words.
+  f_equal.
+  etransitivity; last apply (take_drop sz (drop off ws)).
+  f_equal.
+  unfold get_path_words.
+  rewrite length_take, length_drop.
+  f_equal; lia.
+Qed.
